LogicalRefinement/Tactics.lean
@@ -1,0 +1,45 @@
+import Lean
+
+open Lean Elab.Tactic Meta
+
+-- Adapted from https://github.com/leanprover/lean4/blob/master/src/Lean/Elab/Tactic/BuiltinTactic.lean
+def renameInaccessibles' (mvarId : MVarId) (hs : Array Syntax) : TacticM MVarId := do
+  if hs.isEmpty then
+    return mvarId
+  else
+    let mvarDecl ← getMVarDecl mvarId
+    let mut lctx  := mvarDecl.lctx
+    let mut hs    := hs
+    let mut found : NameSet := {}
+    let n := lctx.numIndices
+    for i in [:n] do
+      let j := n - i - 1
+      match lctx.getAt? j with
+      | none => pure ()
+      | some localDecl =>
+        if localDecl.userName.hasMacroScopes || found.contains localDecl.userName then
+          let h := hs.back
+          if h.isIdent then
+            let newName := h.getId
+            lctx := lctx.setUserName localDecl.fvarId newName
+          hs := hs.pop
+          if hs.isEmpty then
+            break
+        found := found.insert localDecl.userName
+    -- unless hs.isEmpty do
+    --   Lean.Elab.logError m!"too many variable names provided"
+    let mvarNew ← mkFreshExprMVarAt lctx mvarDecl.localInstances mvarDecl.type MetavarKind.syntheticOpaque mvarDecl.userName
+    assignExprMVar mvarId mvarNew
+    return mvarNew.mvarId!
+
+syntax "rename_i'" ident*: tactic
+
+elab_rules : tactic
+  | `(tactic| rename_i' $hs*) => 
+    do replaceMainGoal [← renameInaccessibles' (← getMainGoal) hs]
+
+def test_assumption: A -> A := by {
+  intros;
+  rename_i' a b c d e;
+  first | apply e | apply d | apply c | apply b | apply a
+}
